@prefix schema: <http://schema.org/> .
@prefix xsd:   <http://www.w3.org/2001/XMLSchema#> .
@prefix sdmx:  <http://purl.org/linked-data/sdmx#> .
@prefix rdfs:  <http://www.w3.org/2000/01/rdf-schema#> .
@prefix vcard: <http://www.w3.org/2006/vcard/ns#> .
@prefix geo:   <http://www.opengis.net/ont/geosparql#> .
@prefix dbo:   <http://dbpedia.org/ontology/> .
@prefix qb:    <http://purl.org/linked-data/cube#> .
@prefix sf:    <http://www.opengis.net/ont/sf#> .
@prefix sdmx-measure: <http://purl.org/linked-data/sdmx/2009/measure#> .
@prefix rdf:   <http://www.w3.org/1999/02/22-rdf-syntax-ns#> .
@prefix sdmx-code: <http://purl.org/linked-data/sdmx/2009/code#> .
@prefix lodcom: <http://vocab.lodcom.de/> .
@prefix sdmx-concept: <http://purl.org/linked-data/sdmx/2009/concept#> .
@prefix interval: <http://reference.data.gov.uk/def/intervals/> .
@prefix sdmx-attribute: <http://purl.org/linked-data/sdmx/2009/attribute#> .
@prefix sdmx-dimension: <http://purl.org/linked-data/sdmx/2009/dimension#> .
@prefix dc:    <http://purl.org/dc/terms/> .

lodcom:Teilbereich  rdfs:comment  "The sub borough is a statistical entity in which belong different districts. The sub borough further divides highly populated boroughs." ;
        rdfs:label       "Sub Borough"@en , "Teilbereich"@de ;
        rdfs:subClassOf  dbo:AdministrativeRegion .

lodcom:upperAdministrativeLevel
        a             rdf:Property ;
        rdfs:comment  "relates an administrative region to its next higher administrative level, e.g. districts to sub borough or boroughs." ;
        rdfs:domain   dbo:AdministrativeRegion ;
        rdfs:range    dbo:AdministrativeRegion .

dbo:AdministrativeRegion
        rdfs:subClassOf  "http://www.opengis.net/ont/geosparql#Feature" .

lodcom:districtId  a  rdf:Property ;
        rdfs:comment  "The city administration uses unique identifier for their districts." ;
        rdfs:domain   lodcom:Stadtteil ;
        rdfs:range    xsd:integer .

lodcom:Stadtteil  rdfs:comment  "A city district describes the smallest spatial division in the city administration." ;
        rdfs:label       "City District"@en , "Stadtteil"@de ;
        rdfs:subClassOf  dbo:AdministrativeRegion .

lodcom:Stadtbezirk  rdfs:comment  "The borough is the largest spatial administrative region in the city administration." ;
        rdfs:label       "Borough"@en , "Stadtbezirk"@de ;
        rdfs:subClassOf  dbo:AdministrativeRegion .
